breaking ground on statement typing

deps/poulet4/lib/Semantics.v
@@ -1338,13 +1338,13 @@ Inductive exec_stmt (read_one_bit : option bool -> bool -> Prop) :
     (if is_continue sig then exec_write st lv sv st' else st' = st) ->
     exec_stmt read_one_bit this_path st
               (MkStatement tags (StatAssignment lhs rhs) typ) st' sig
-| exec_stmt_assign_func_call : forall lhs lv rhs sv this_path
+| exec_stmt_assign_func_call : forall lhs lv rhs this_path
                                  st tags typ st' st'' sig sig' ret_sig,
     exec_call read_one_bit this_path st rhs st' sig' ->
     exec_lexpr read_one_bit this_path st lhs lv sig ->
-    (if not_continue sig then st'' = st /\ ret_sig = sig /\ sv = Value.ValBaseNull
-     else if not_return sig' then st'' = st' /\ ret_sig = sig' /\ sv = Value.ValBaseNull
-          else get_return_sval sig' sv /\
+    (if not_continue sig then st'' = st /\ ret_sig = sig
+     else if not_return sig' then st'' = st' /\ ret_sig = sig'
+          else exists sv, get_return_sval sig' sv /\
                exec_write st' lv sv st'' /\ ret_sig = SContinue) ->
     exec_stmt read_one_bit this_path st
               (MkStatement tags (StatAssignment lhs rhs) typ) st'' ret_sig
